extraction/theories/AnalyzeCorrectness.v
@@ -1,0 +1,124 @@
+From ConCert.Extraction Require Import Aux.
+From ConCert.Extraction Require Import ExTyping.
+From ConCert.Extraction Require Import Optimize.
+From ConCert.Extraction Require Import OptimizeCorrectness.
+From Coq Require Import Arith.
+From Coq Require Import Btauto.
+From Coq Require Import Bool.
+From Coq Require Import List.
+From Equations Require Import Equations.
+From MetaCoq.Erasure Require Import EInduction.
+From MetaCoq.Template Require Import utils.
+Import ListNotations.
+Import ExAst.
+Open Scope bool.
+
+Lemma get_mib_masks_ne p im kn :
+  fst p <> kn ->
+  get_mib_masks (p :: im) kn = get_mib_masks im kn.
+Proof.
+  intros ne.
+  unfold get_mib_masks.
+  destruct p; cbn in *.
+  unfold eq_kername.
+  now destruct (kername_eq_dec _ _).
+Qed.
+
+Lemma valid_case_masks_add_new Σ kn brs im ind npars m :
+  lookup_env Σ kn = None ->
+  inductive_mind ind <> kn ->
+  Forall (fun br => wfe_term Σ br.2) brs ->
+  valid_case_masks im ind npars brs ->
+  valid_case_masks ((kn, m) :: im) ind npars brs.
+Proof.
+  intros no_prev ne wf_brs valid_brs.
+  unfold valid_case_masks in *.
+  now rewrite get_mib_masks_ne.
+Qed.
+
+Lemma valid_proj_add_new Σ kn im ind npars arg m :
+  lookup_env Σ kn = None ->
+  inductive_mind ind <> kn ->
+  valid_proj im ind npars arg ->
+  valid_proj ((kn, m) :: im) ind npars arg.
+Proof.
+  intros no_prev ne valid_p.
+  unfold valid_proj.
+  now rewrite get_mib_masks_ne.
+Qed.
+
+Lemma valid_cases_add_new Σ kn t im m :
+  lookup_env Σ kn = None ->
+  wfe_term Σ t ->
+  valid_cases im t ->
+  valid_cases ((kn, m) :: im) t.
+Proof.
+  intros no_prev wf_t valid_t.
+  induction t using term_forall_list_ind; cbn in *; propify; auto; try tauto.
+  - induction H; [easy|].
+    cbn in *.
+    now propify.
+  - destruct p.
+    propify.
+    apply and_assoc.
+    split; [easy|].
+    split; cycle 1.
+    + unfold lookup_minductive in *.
+      destruct (lookup_env Σ (inductive_mind i)) eqn:ind_found; [|easy].
+      eapply valid_case_masks_add_new; [eassumption|congruence| |easy].
+      now apply forallb_Forall.
+    + destruct valid_t as ((_ & valid_brs) & _).
+      destruct wf_t as (_ & wf_brs).
+      induction X; [easy|].
+      cbn in *.
+      propify; split; [easy|].
+      now apply IHX.
+  - destruct s as ((ind & npars) & arg).
+    propify; split; [easy|].
+    unfold lookup_minductive in *.
+    destruct (lookup_env Σ (inductive_mind ind)) eqn:ind_found; [|easy].
+    now eapply valid_proj_add_new.
+  - induction H; [easy|].
+    cbn in *; propify.
+    now rewrite H.
+  - induction H; [easy|].
+    cbn in *; propify.
+    now rewrite H.
+Qed.
+
+Lemma valid_masks_decl_add_new Σ kn im cm m :
+  lookup_env Σ kn = None ->
+  wfe_env Σ ->
+  valid_masks_env im cm Σ ->
+  forallb (valid_masks_decl ((kn, m) :: im) cm) Σ.
+Proof.
+  intros no_prev wfe valid.
+  induction Σ as [|(kn', decl) Σ IH]; [easy|].
+  cbn in *.
+  unfold eq_kername in no_prev.
+  destruct (kername_eq_dec _ _); [easy|].
+  destruct decl; cbn in *; propify; [|easy|easy].
+  destruct c.
+  destruct cst_body; cbn in *; [|easy].
+  propify.
+  split; [|easy].
+  split; [easy|].
+  now eapply valid_cases_add_new.
+Qed.
+
+Lemma analyze_correct Σ :
+  wfe_env Σ ->
+  let (consts, inds) := analyze_env Σ in
+  valid_masks_env inds consts Σ.
+Proof.
+  intros wfe.
+  induction Σ as [|(kn, decl) Σ IH]; [easy|].
+  cbn in *.
+  propify.
+  specialize (IH (proj2 wfe)).
+  destruct (analyze_env Σ).
+  destruct decl; cycle 1; cbn.
+  - destruct lookup_env eqn:no_prev; [easy|].
+    now apply valid_masks_decl_add_new.
+  - easy.
+  -
