extraction/theories/ErasureCorrectness.v
@@ -1,0 +1,14 @@
+From ConCert.Extraction Require Import Aux.
+From ConCert.Extraction Require Import Erasure.
+From ConCert.Extraction Require Import ExTyping.
+From ConCert.Extraction Require Import Optimize.
+From ConCert.Extraction Require Import OptimizeCorrectness.
+From Coq Require Import Arith.
+From Coq Require Import Btauto.
+From Coq Require Import Bool.
+From Coq Require Import List.
+From Equations Require Import Equations.
+From MetaCoq.Erasure Require Import EInduction.
+From MetaCoq.Template Require Import utils.
+Import ListNotations.
+Open Scope bool.
